\section{Dual Vector Spaces}

\begin{definition}
Let \(V \in \Obj(\Vect_k)\), then, we define the dual vector space of
\(V\) to be
\[
  V^\ast = \Hom_{\Vect_k} (V, k)
\]
and \(f \in V^\ast\) is called a linear functional on \(V\).
\end{definition}

\begin{proposition}
For all sets \(S\) there exists a natural isomorphism between the dual free
vector space generated by \(S\) and the function space \(S \to k\), that is
\[
  (k^{\oplus S})^\ast \iso k^S.
\]
\end{proposition}

\begin{proof}
This result comes directly from the free vector space universal property, that
is
\[
  \begin{tikzcd}
    S \ar[r, "f"] \ar[d, tail] & k \\
    k^{\oplus S} \ar[ur, dashed, swap, "\ell"]
  \end{tikzcd}
\]
so that we can assign for each function \(f \in k^S\) the corresponding unique
\(k\)-linear morphism \(\ell \in (k^{\oplus S})^\ast\).
\end{proof}

\begin{proposition}\label{prop: finite dim vs iso dual vs}
Let \(V\) be finite dimensional, then there exists a non-canonical isomorphism
\[
  V \iso V^\ast
\]
\end{proposition}

\begin{proof}
The proof here is rather arbitrary, we'll just construct explicitly an
isomorphism by defining an ordered basis \(B = (v_1, \dots, v_n)\) of \(V\),
but we could build other isomorphisms (this is why the proposition states
``non-canonical''). Define the \(k\)-linear morphism \(\varphi(v_i) = e_i\)
where \(e_i\) is the \(i\)-th standard basis on \(k^n\), then \(\varphi\) is
an isomorphims \(V \iso k^n\). Moreover, from the standard inner product, we
have that \(k^n \iso (k^n)^\ast\), thus we are done, since
\[
  \begin{tikzcd}
    V \ar[r, "\varphi"] & k^n \iso (k^n)^\ast \ar[r, "f \mapsto f
    \varphi"] &V^\ast
  \end{tikzcd}
\]
thus indeed \(V \iso V^\ast\).
\end{proof}

\begin{proposition}
If \(V\) is finite-dimensional, then \(V^\ast\) is also finite dimensional and
\[
  \dim_k(V) = \dim_k (V^\ast).
\]
\end{proposition}

\begin{proposition}
Given \(k\)-vector spaces \(V\) and \(W\), there exists a natural isomorphism
\[
  (V \oplus W)^\ast \iso V^\ast \oplus W^\ast.
\]
\end{proposition}

\begin{proof}
Consider the mapping \(\Phi: (V \oplus W)^\ast \to V^\ast \oplus W^\ast\)
defined by \(\Phi(f^\ast) = (f^\ast_V, f^\ast_W)\), where \(f^\ast_V =
f^\ast|_{V \oplus \{0\}} \) and \(f^\ast_W = f^\ast|_{\{0\} \oplus W}\). We
now show that \(\Phi\) is an isomorphism. (Injective) Suppose \(g^\ast \in
\ker \Phi\), then necessarily \(g^\ast|_{V\oplus \{0\}} = 0\) and
\(g^\ast|_{\{0\} \oplus W} = 0\), but since \(g^\ast = g^\ast|_{V\oplus
\{0\}} + g^\ast|_{\{0\} \oplus W}\) we conclude that \(g^\ast = 0\).
(Surjective) Let any \((\ell^\ast, t^\ast) \in V^\ast \oplus W^\ast\), then
define the function \(f^\ast \in (V \oplus W)^\ast\) such that \(f^\ast(v, w)
= \ell^\ast(v) + t^\ast(w)\), then \(f^\ast|_{V \oplus \{0\}} = \ell^\ast\)
and \(f^\ast|_{\{0\} \oplus W} = t^\ast\), therefore \(\Phi(f^\ast) =
(\ell^\ast, t^\ast)\).
\end{proof}

\begin{definition}\label{def:dual-morphism}
Let \(f : V \to W\) be a \(k\)-linear morphism. We define the dual (or
transpose) \(k\)-linear morphism of \(f\) as \(f^\ast = f^T : W^\ast \to
V^\ast\). This is a particular case of the induced \(\Hom\) \(k\)-linear
morphism, by taking the \(k\)-vector space \(k\), so that
\[
  f^\ast : \Hom(W, k) \to \Hom(V, k),\ \alpha \mapsto \alpha  f.
\]
It is immediate from this definition that \((g f)^{*} = f^{*} g^{*}\) for
every composable pair of functionals \(f\) and \(g\).
\end{definition}

\begin{proposition}
Let \(f : V \to W\) be a \(k\)-linear morphism and consider its dual \(f^\ast
: W^\ast \to V^\ast\). If \(f\) is injective, then \(f^\ast\) is surjective,
on the other hand, if \(f\) is surjective, then \(f^\ast\) is injective.
Hence, if \(f\) is an isomorphism, then \(f^*\) is an isomorphism.
\end{proposition}

\begin{proposition}
Let \(V_1 \to V_2 \to V_3\) be an exact sequence, then \(V_3^\ast \to
V_2^\ast \to V_1^\ast\) is also exact.
\end{proposition}

\begin{proof}
Let \(f: V_1 \to V_2\) and \(g: V_2 \to V_3\) be such that \(\im(f) =
\ker(g)\). Then, given any \(\alpha \in V_3^\ast\) and consider
\(g^\ast(\alpha) = \alpha  g\), we then have \(f^\ast(\alpha  g) =
(\alpha  g)  f = \alpha  (g  f) = 0\) from the
construction of \(f, g\), thus \(\im(g^\ast) \subseteq \ker(f^\ast)\). On the
other hand, let \(\beta \in \ker(f^\ast) \subseteq V_2^\ast\) so that
\(f^\ast(\beta) = \beta  f = 0\), which is the same thing as requiring
\(\beta|_{\im(f)} = 0\); this way we can see that for any element \(\alpha \in
V_3^\ast\) we have \(g^\ast(\alpha) = \alpha  g\) be such that \(\alpha
  g|_{\im(f)} = 0\) since \(\ker(g) = \im(f)\) and thus already satisfies
as an element of the kernel of \(f^\ast\), therefore \(\ker(f^\ast) \subseteq
\im(g^\ast)\).
\end{proof}

\begin{proposition}
Let \(V_1 \to V_2 \to V_3\) be exact sequence of \(k\)-vector spaces, then for
any given \(k\)-vector space \(W\) we have that
\[
  \Hom(V_3, W) \longrightarrow \Hom(V_2, W) \longrightarrow \Hom(V_1, W)
\]
is exact (contravariant \(\Hom\)).
\end{proposition}

\begin{proof}
The proof is almost identical to the latter.
\end{proof}

\begin{proposition}
Let \(V_1 \to V_2 \to V_3\) be exact sequence of \(k\)-vector spaces, then for
any given \(k\)-vector space \(W\) we have that
\[
  \Hom(W, V_1) \longrightarrow \Hom(W, V_2) \longrightarrow \Hom(V_3, W)
\]
is exact (covariant \(\Hom\)).
\end{proposition}

\begin{proof}
The proof only diverges from the above because we have the mappings
\(g_\ast(\alpha) = g  \alpha\) and \(f_\ast(\beta) = f  \beta\).
\end{proof}

\begin{proposition}
Consider a \(k\)-linear morphism \(f : V \to W\) such that \(\mathrm{rank}(f)\) is
finite (that is, \(\dim_k(\im(f))\) exists). Then \(\mathrm{rank}(f) =
\mathrm{rank}(f^\ast)\).
\end{proposition}

\begin{proof}
Notice that if \(f : V \epi U \mono W\) is the
decomposition of \(f\), then we can consider the dual \(f^\ast: W^\ast \to
V^\ast\) as having a decomposition \(W^\ast \epi U^\ast
\mono V^\ast\), since the dual of an injective map is surjective and
the dual of a surjective map is injective. Therefore, given a basis \(B\) for
\(U\), since \(\forall b \in B\) there exists \(v \in V\) for which \(f(v) =
b\) we can say that \(b \in \im(f)\) and, moreover, \(\rank(f) \geq
\dim_k(U)\). Also, since \(\im(f) \subseteq U\), then we have directly that
\(\rank(f) \leq \dim_k(U)\), thus \(\rank(f) = \dim_k(U)\). The same shows
that \(\rank(f^\ast) = \dim_k(U^\ast)\) and since \(U \iso U^\ast\) we find
that \(\dim_k(U) = \dim_k(U^\ast)\) and hence \(\rank(f) = \rank(f^\ast)\).
\end{proof}

\begin{proposition}\label{prop: dual matrix equals transpose}
Let \(\ell \in \Hom(V, W)\), where \(V \iso k^n\) and \(W \iso k^m\), so that
\(\ell\) can be written as a matrix \(L : k^n \to k^m\). Then the dual
\(\ell^\ast\) is represented by the matrix \(L^T\).
\end{proposition}

\begin{proof}
Define \((v_j)_{j=1}^n\) an ordered basis for \(V\) and \((v_i^\ast)_{i=1}^n\)
be its dual ordered basis; define also \((w_i)_{i=1}^m\) to be an ordered
basis for \(W\) and \((w_j^\ast)_{j=1}^m\) be its dual ordered basis. Notice
that the dual of the matrix, that is, \(L^\ast : (k^m)^\ast \to (k^n)^\ast\)
can be written as \(L^\ast : k^m \to k^n\), since \((k^m)^\ast \iso k^m\) and
\((k^n)^\ast \iso k^n\). Define the representations
\[
  L =
  \begin{bmatrix}
    t_{1, 1} & \dots   & t_{1, n} \\
    \vdots   & \ddots  & \vdots   \\
    t_{m, 1} & \dots   & t_{m, n}
  \end{bmatrix}
  \ \text{ and define }\
  L^\ast =
  \begin{bmatrix}
    d_{1, 1} & \dots   & d_{1, m} \\
    \vdots   & \ddots  & \vdots   \\
    d_{n, 1} & \dots   & d_{n, m}
  \end{bmatrix}
\]
By definition of the dual linear morphism, we have \(L^\ast(w_j^\ast) =
w_j^\ast  L\). When this transformation is thought of as a \(k^n \to
k^m\) matrix, the definition of a matrix for a linear transformation with
respect to the given dual basis for \(W^\ast\) and \(V^\ast\) is defined such
that \(L^\ast(w_j^\ast) = \sum_{r = 1}^n d_{r, j} v_r^\ast\). Hence, given any
element \(v_k \in (v_j)_{j=1}^n \subseteq V\), from the first definition:
\begin{equation}
  w_j^\ast  L (v_k)
  = w_j^\ast \left( \sum_{r=1}^m t_{r, k} w_r \right)
  = \sum_{r=1}^m t_{r, k} w_j^\ast(w_r)
  = t_{j, k}
\end{equation}
from the fact that we defined \(w_j^\ast\) so that \(w_j^\ast(w_j) = 1\) and
\(w_j^\ast(w_i) = 0\) for \(i \neq j\). Now, from the second definition that
we discussed, we have (applying the same \(v_k\)):
\begin{equation}
  \sum_{r=1}^n d_{r,j} v_r^\ast(v_k)
  = d_{k, j}
\end{equation}
from the same fact. Thus we conclude that \(d_{k,j} = t_{j,k}\) for all \(1
\leq k \leq n\) and \(1 \leq j \leq m\), thus indeed \(L^\ast = L^T\)
\end{proof}

\begin{definition}[Column and Row Rank]\label{def: column and row rank}
Let \(L: k^n \to k^m\) be a matrix. Define \((v_j)_{j=1}^n\) to be the vectors
whose components are given by the ordered \(j\)-th column elements of the
matrix representation of \(L\). Analogously, define \((w_i)_{i=1}^m\) to be
the vectors whose components are the ordered \(i\)-th row elements of the
matrix representation of \(L\). We define the column rank of \(L\) to be
\(\dim_k(\mathrm{span}(v_j)_{j=1}^n)\) and the row rank of \(L\) to be
\(\dim_k(\mathrm{span}(w_i)_{i=1}^m)\).
\end{definition}

\begin{proposition}
\label{prop: column and row rank equal the rank}
Let \(L: V \to W\) be a linear morphism with \(V \iso k^n\) and \(W \iso
k^m\), its row and column rank of its matrix representation \(k^n \to k^m\)
are both equal to the rank of \(L\).
\end{proposition}

\begin{proof}
Let \((v_j)_{j=1}^n\) and  \((w_i)_{i=1}^m\) be the column and row vectors of
the matrix representation of \(L\).
(Rank equals column rank) Let \(B_V\) and \(S_W\) be ordered basis for \(V\)
and \(W\) respectively and any element \(w \in \im(L) = \mathrm{span}(Lb_k :
b_k \in B_V)\) notice that since \(Lb_k = \sum_{i=1}^m t_{i, k} s_i\), where
\(t_{i,j}\) are the elements of the matrix representation of \(L\), then we
see that \(Lb_k\) is a linear combination of the \(k\)-th column vector of
\(L\), hence \(Lb_k \in \mathrm{span}(v_j)_{j=1}^n\) for all \(1 \leq k \leq
m\). Therefore we conclude that \(w \in \mathrm{span}(v_i)_{i=1}^n\).
Moreover, we have \(\mathrm{span}(v_i)_{i=1}^n \subseteq \im(L)\), thus
\(\mathrm{span}(v_i)_{i=1}^n = \im(L)\), hence we conclude finally that
\(\dim_k(\im(L)) = \rank(L) = \dim_k(\mathrm{span}(v_i)_{i=1}^n)\) which
states that the rank of \(L\) equals the column rank.
(Rank equals column rank) Notice that \(L^\ast : (k^m)^\ast \to (k^n)^\ast\)
is isomorphic to the matrix \(k^m \to k^n\) and the matrix representation of
the dual of \(L\) is equal to its transpose by \ref{prop: dual matrix equals
transpose}, moreover we proved lastly that the column rank of a matrix equals
its rank, thus it should be true that \(\rank(L^\ast) =
\dim_k(\mathrm{span}(w_i)_{i=1}^m)\). Since \(L^\ast \iso L\), it follows that
\(\rank(L) = \dim_k(\mathrm{span}(w_i)_{i=1}^m)\). Hence we conclude that
\[
  \rank(L) = \rank(\text{column}) = \rank(\text{row}).
\]
\end{proof}

\begin{definition}[Bilinear map]\label{def: bilinear map}
A map \(V^\ast \times V \to k\) that has the mapping \((\alpha, v) \mapsto
\alpha(v)\) is called a bilinear map. This map is linear only when we fix the
second component to some \(v \in V\) so that \(f_v: V^\ast \to k\) with the
mapping \(\alpha \mapsto \alpha(v)\) is a \(k\)-linear morphism.
\end{definition}

This defines a rather interesting canonical \(k\)-linear morphism
\[
\Psi_V : V \to (V^\ast)^\ast,\
\text{ mapping }\ v \mapsto (f_v = (\alpha \mapsto \alpha(v))).
\]

\begin{proposition}
The morphism \(\Psi_V\) is an injection for every given vector space \(V\).
\end{proposition}

\begin{proposition}
A finite dimensional space \(V\) is isomorphic to its double dual
\(V^{\ast\ast}\). The same can't be said if \(V\) is infinite dimensional.
\end{proposition}

\begin{proof}
Let \(\{v_i\}_{i=1}^n\) be a basis for \(V\), \(\{v_i^\ast\}_{i=1}^n\) be a
basis for \(V^\ast\) dual to the first given basis, and
\(\{v_i^{\ast\ast})_{i=1}^n\}\) be a basis for \(V^{\ast\ast}\) dual to the
second given basis. We'll show that \(\Psi_V(v_i) = v_i^{\ast\ast}\). Let
\(v_i\) be an element of the given basis of \(V\), then, we know from the
definition of the dual of the basis that \(v_k^\ast(v_i) = \delta_{i, k}\) and
\(v_t^{\ast\ast}(v_k^\ast) = \delta_{k, t}\).  Moreover, since \(\Psi_V\) is
an injection, we see that if \(\Psi_V(v_i) \neq 0\), hence \(v_i \mapsto
v_i^{\ast\ast}\), which proves the statement.
\end{proof}

\begin{definition}[Annihilator]\label{def: annihilator}
Let \(V\) be a finite dimensional \(k\)-vector space and \(W\) be a subspace
of \(V\). The annihilator of \(W\) is defined as the subspace of \(V^\ast\)
given by
\[
  W^0 = \{\alpha \in V^\ast \colon \alpha(W) = 0\}.
\]
\end{definition}

\begin{proposition}
Let \(V\) be a finite dimensional space and \(W \subseteq V\) a subspace. Then
\[
  \dim_k(V) = \dim_k(W) + \dim_k(W^0).
\]
\end{proposition}

\begin{proof}
Let the inclusion \(\iota : W \emb V\), then its dual \(\iota^\ast :
V^\ast \epi W^\ast\) is surjective. Moreover, let \(\alpha \in
W^0\) then, \(\iota^\ast(\alpha) = \alpha  \iota\), since \(\im(\iota)
\subseteq W\) we conclude that \(\iota^\ast(\alpha) = 0\) and thus \(\alpha
\in \ker(\iota^\ast)\), so that \(W^0 \subseteq \ker(\iota^\ast)\). Moreover,
if \(\alpha \in \ker(\iota^\ast)\) then, in particular, \(\alpha(W) = 0\)
hence \(\alpha \in W^0\). Then we find that \(W^0 = \ker(\iota^\ast)\). We now
use the theorem \ref{thm: rank plus nullity} on the morphism \(\iota^\ast\) so
that \(\dim_k(V^\ast) = \dim_k(\ker(\iota^\ast)) + \rank(\iota^\ast)\). Since
\(\iota^\ast\) is surjective, then \(\im(\iota^\ast) = W^\ast\) and therefore
\(\rank(\iota^\ast) = \dim_k(W^\ast)\); moreover, \(\dim_k(\ker(\iota^\ast)) =
\dim_k(W^0)\); and finally \(\dim_k(V^\ast) = \dim_k(V)\), and
\(\dim_k(W^\ast) = \dim_k(W)\). Thus indeed \(\dim_k(V) = \dim_k(W) +
\dim_k(W^0)\).
\end{proof}
